update some more loops to new invariant style

pulse/lib/pulse/lib/Pulse.Lib.HashTable.fst
@@ -106,10 +106,8 @@ fn lookup
   let mut ret = None #SZ.t;
   unfold (models ht pht);
 
-  while (let voff = !off;
-         let vcont = !cont;
-         (voff <=^ ht.sz && vcont = true))
-  invariant b. exists* (voff:SZ.t) (vcont :bool) vcontents. (
+  while ((!off <=^ ht.sz && !cont))
+  invariant exists* (voff:SZ.t) (vcont :bool) vcontents. (
     pts_to contents vcontents **
     V.pts_to vcontents pht.repr.seq **
     pts_to off voff **
@@ -120,8 +118,7 @@ fn lookup
       V.is_full_vec vcontents /\
       voff <=^ ht.sz /\
       walk_get_idx pht.repr (SZ.v cidx) k (SZ.v voff)
-        == lookup_repr_index pht.repr k /\
-      b == (voff <=^ ht.sz && vcont = true)
+        == lookup_repr_index pht.repr k
     ))
   {
     let voff = !off;
@@ -268,12 +265,8 @@ fn insert
   let mut cont = true;
   let mut idx = 0sz;
 
-  while
-  (
-    let vcont = !cont;
-    (vcont = true)
-  )
-  invariant b. exists* (voff:SZ.t) (vcont :bool) (vcontents:V.vec _) vidx s. (
+  while ((!cont))
+  invariant exists* (voff:SZ.t) (vcont :bool) (vcontents:V.vec _) vidx s. (
     pts_to off voff **
     pts_to cont vcont **
     pts_to idx vidx **
@@ -293,9 +286,7 @@ fn insert
         (insert_repr #kt #vt #(pht_sz pht) #pht.spec pht.repr k v).seq `Seq.equal`
         Seq.upd s (SZ.v vidx) (mk_used_cell k v))) /\
 
-      ((vcont) ==> s `Seq.equal` pht.repr.seq) /\  // insert failed
-
-      b == (vcont = true)
+      ((vcont) ==> s `Seq.equal` pht.repr.seq)
     ))
   {
     let voff = !off;
@@ -547,11 +538,9 @@ fn delete
 
   while
   (
-    let vcont = !cont;
-    let verr = !err;
-    (vcont = true && verr = false)
+    (!cont && not (!err))
   )
-  invariant b. exists* (voff:SZ.t) (vcont verr:bool) (contents_v:V.vec _). (
+  invariant exists* (voff:SZ.t) (vcont verr:bool) (contents_v:V.vec _). (
     pts_to off voff **
     pts_to cont vcont **
     pts_to err verr **
@@ -564,8 +553,7 @@ fn delete
       all_used_not_by pht.repr (SZ.v cidx) (SZ.v voff) k /\
       walk pht.repr (SZ.v cidx) k (SZ.v voff) == lookup_repr pht.repr k /\
       delete_repr_walk #kt #vt #(pht_sz pht) #pht.spec pht.repr k (SZ.v voff) (SZ.v cidx) () ()
-        == delete_repr #kt #vt #(pht_sz pht) #pht.spec pht.repr k /\
-      b == (vcont = true && verr = false)
+        == delete_repr #kt #vt #(pht_sz pht) #pht.spec pht.repr k
     ))
   {
     with vcont. assert (pts_to cont vcont);
